One more round of changes in heap definitions pt.2

theories/L6_PCPS/Heap/heap_defs.v
@@ -121,13 +121,13 @@ Module HeapDefs (H : Heap).
     forall l, l \in S -> exists v, get l H = Some v /\ locs v \subset S.
 
   (** Add a block of function definitions in the heap and the environment *)
-  Fixpoint def_closures (B B0: fundefs) (rho : env) (H : heap block) (ct : cTag) (cenv : loc) {struct B}
+  Fixpoint def_closures (B B0: fundefs) (rho : env) (H : heap block) (cenv : loc) {struct B}
   : heap block * env :=
     match B with
       | Fcons f _ _ _ B' =>
-        let '(H', rho') := def_closures B' B0 rho H ct cenv in
+        let '(H', rho') := def_closures B' B0 rho H cenv in
         (* construct the closure *)
-        let clo := Constr ct [FunPtr B0 f ; Loc cenv] in
+        let clo := Clos (FunPtr B0 f) (Loc cenv) in
         (* add it to heap *)
         let '(l, H'') := alloc clo H' in
         (* extend the environment *)
@@ -597,14 +597,14 @@ Module HeapDefs (H : Heap).
   Qed.
 
   
-  Lemma def_closures_env_locs_in_dom S H H' rho rho' B B0 ct l :
-    def_closures B B0 rho H ct l = (H', rho') ->
+  Lemma def_closures_env_locs_in_dom S H H' rho rho' B B0 l :
+    def_closures B B0 rho H l = (H', rho') ->
     env_locs rho S \subset dom H ->
     env_locs rho' (S :|: name_in_fundefs B) \subset dom H'.
   Proof.
     revert S rho rho' H H'; induction B; intros S rho rho' H H' Hdef Hsub; simpl.
     - simpl in Hdef.
-      destruct (def_closures B B0 rho H ct l) as [H'' rho''] eqn:Hdef'.
+      destruct (def_closures B B0 rho H l) as [H'' rho''] eqn:Hdef'.
       destruct (alloc _ H'') as [l' H'''] eqn:Hal. inv Hdef.
       rewrite alloc_dom; [| eassumption ].
       rewrite env_locs_set_In; [| now eauto with Ensembles_DB ].
@@ -616,14 +616,14 @@ Module HeapDefs (H : Heap).
     - rewrite Union_Empty_set_neut_r. inv Hdef. eassumption.
   Qed.
 
-  Lemma env_locs_def_funs S S1 H1 H1' rho1 rho1'  B B0 c l :
+  Lemma env_locs_def_funs S S1 H1 H1' rho1 rho1'  B B0 l :
     env_locs rho1 (Setminus _ S (name_in_fundefs B)) \subset S1 ->
     l \in S1 ->
-    (H1', rho1') = def_closures B B0 rho1 H1 c l ->
+    (H1', rho1') = def_closures B B0 rho1 H1 l ->
     env_locs rho1' (Setminus _ S (name_in_fundefs B)) \subset S1.
   Proof.
     revert S H1' rho1'; induction B; intros S H1' rho1' Hsub1 Hsub2 Heq.
-    - simpl in Heq. destruct (def_closures B B0 rho1 H1 c l) as [H'' rho''].
+    - simpl in Heq. destruct (def_closures B B0 rho1 H1 l) as [H'' rho''].
       destruct (alloc _ H'') as [l' H'''] eqn:Heq'.
       inv Heq. rewrite env_locs_set_not_In.
       simpl; rewrite <- !Setminus_Union.
@@ -854,13 +854,13 @@ Module HeapDefs (H : Heap).
 
   (** * Lemmas about [def_closures] *)
 
-  Lemma def_funs_subheap H H' rho rho' B B0 c l :
-    (H', rho') = def_closures B B0 rho H c l ->
+  Lemma def_funs_subheap H H' rho rho' B B0 l :
+    (H', rho') = def_closures B B0 rho H l ->
     H ⊑ H'.
   Proof.
     revert H' rho'; induction B; intros H' rho' Heq;
     simpl; [| inv Heq; now apply subheap_refl ].
-    simpl in Heq. destruct (def_closures B B0 rho H c l) as [H'' rho''].
+    simpl in Heq. destruct (def_closures B B0 rho H l) as [H'' rho''].
     destruct (alloc _ H'') as [l' H'''] eqn:Heq'.
     inv Heq. eapply subheap_trans; eauto.
     now eapply alloc_subheap; eauto.
@@ -869,14 +869,14 @@ Module HeapDefs (H : Heap).
 
   Lemma def_closures_post_reach
         (S : Ensemble var) (H H' : heap block) (rho rho' : env)
-        (B B0 : fundefs) (ct : cTag) (l : loc) :
-    def_closures B B0 rho H ct l = (H', rho') ->
+        (B B0 : fundefs) (l : loc) :
+    def_closures B B0 rho H l = (H', rho') ->
     post H [set l] \subset (reach' H (env_locs rho S)) ->
     post H' [set l] \subset (reach' H' (env_locs rho' (S :|: name_in_fundefs B))).
   Proof.
     revert S rho rho' H H'; induction B; intros S rho rho' H H' Hdef Hsub; simpl.
     - simpl in Hdef.
-      destruct (def_closures B B0 rho H ct l) as [H'' rho''] eqn:Hdef'.
+      destruct (def_closures B B0 rho H l) as [H'' rho''] eqn:Hdef'.
       destruct (alloc _ H'') as [l' H'''] eqn:Hal. inv Hdef.
       intros l1 [l2 [b2 [Hin1 [Hget2 Hin2]]]]. inv Hin1. 
       exists 2. split. constructor.
@@ -885,27 +885,27 @@ Module HeapDefs (H : Heap).
       eexists v. split. right. left. reflexivity.
       rewrite M.gss. reflexivity.
       split. eapply gas; eassumption.
-      simpl. right. left. reflexivity.
+      simpl. right. reflexivity.
       split; eauto.
     - rewrite Union_Empty_set_neut_r. inv Hdef.
       eassumption.
   Qed.
 
-  Lemma def_closures_env_reach S H H' rho rho' B B0 ct l :
-    def_closures B B0 rho H ct l = (H', rho') ->
+  Lemma def_closures_env_reach S H H' rho rho' B B0 l :
+    def_closures B B0 rho H l = (H', rho') ->
     l \in (reach' H (env_locs rho S)) ->
     l \in (reach' H' (env_locs rho' (S :|: name_in_fundefs B))).
   Proof.
     revert S rho rho' H H'; induction B; intros S rho rho' H H' Hdef Hin; simpl.
     - simpl in Hdef.
-      destruct (def_closures B B0 rho H ct l) as [H'' rho''] eqn:Hdef'.
+      destruct (def_closures B B0 rho H l) as [H'' rho''] eqn:Hdef'.
       destruct (alloc _ H'') as [l' H'''] eqn:Hal. inv Hdef.
       exists 1. split. constructor.
       exists l'. eexists. split. simpl.
       eexists v. split. right. left. reflexivity.
       rewrite M.gss. reflexivity.
       split. eapply gas; eassumption.
-      simpl. right. left. reflexivity.
+      simpl. right. reflexivity.
     - rewrite Union_Empty_set_neut_r. inv Hdef.
       eassumption.
   Qed.
@@ -1041,32 +1041,32 @@ Module HeapDefs (H : Heap).
       eexists. erewrite gao; eauto; split; eauto...
   Qed.
 
-  Lemma closed_def_funs S1 H1 H1' rho1 rho1'  B B0 c l :
+  Lemma closed_def_funs S1 H1 H1' rho1 rho1'  B B0 l :
     closed S1 H1 ->
     l \in S1 ->
-    (H1', rho1') = def_closures B B0 rho1 H1 c l ->
+    (H1', rho1') = def_closures B B0 rho1 H1 l ->
     closed S1 H1'.
   Proof.
     revert H1' rho1'; induction B;
     intros H1' rho1' Hc Hsub Heq; [| inv Heq; now eauto ].
-    simpl in Heq. destruct (def_closures B B0 rho1 H1 c l) as [H'' rho''].
+    simpl in Heq. destruct (def_closures B B0 rho1 H1 l) as [H'' rho''].
     destruct (alloc _ H'') as [l' H'''] eqn:Heq'.
     inv Heq. eapply closed_alloc'; [| | eassumption ]; eauto.
-    simpl. rewrite Union_Empty_set_neut_r, Union_Empty_set_neut_l.
+    simpl. rewrite Union_Empty_set_neut_l.
     eapply Singleton_Included. eassumption.
   Qed.
   
-  Lemma def_funs_exists_new_set S S1 H1 H1' rho1 rho1' rho_clo B B0 c l :
+  Lemma def_funs_exists_new_set S S1 H1 H1' rho1 rho1' rho_clo B B0 l :
     closed S1 H1 ->
     env_locs rho1 (Setminus _ S (name_in_fundefs B)) \subset S1 ->
     get l H1 = Some (Env rho_clo) ->
     env_locs rho_clo (Full_set _) \subset S1 ->
-    (H1', rho1') = def_closures B B0 rho1 H1 c l ->
+    (H1', rho1') = def_closures B B0 rho1 H1 l ->
     exists S1', S1 \subset S1' /\ closed S1' H1' /\
            env_locs rho1' S \subset S1'.
   Proof with now eauto with Ensembles_DB.
     revert S H1' rho1'; induction B; intros S H1' rho1' Hc Henv Hget Hsub Heq.
-    - simpl in Heq. destruct (def_closures B B0 rho1 H1 c l) as [H'' rho''] eqn:Hdef.
+    - simpl in Heq. destruct (def_closures B B0 rho1 H1 l) as [H'' rho''] eqn:Hdef.
       destruct (alloc _ H'') as [l' H'''] eqn:Heq'.
       inv Heq.
       edestruct IHB as [S1' [Hsub' [Hc' Henv']]]; eauto.
@@ -1316,18 +1316,18 @@ Module HeapDefs (H : Heap).
     rewrite reach'_Union. eapply well_formed_Union; eauto.
   Qed.
   
-  Lemma well_formed_def_funs S1 H1 H1' rho1 rho1'  B B0 c l :
+  Lemma well_formed_def_funs S1 H1 H1' rho1 rho1'  B B0 l :
     well_formed S1 H1 ->
     l \in dom H1 ->
-    (H1', rho1') = def_closures B B0 rho1 H1 c l ->
+    (H1', rho1') = def_closures B B0 rho1 H1 l ->
     well_formed S1 H1'.
   Proof.
     revert H1' rho1'; induction B;
     intros H1' rho1' Hc Hsub Heq; [| inv Heq; now eauto ].
-    simpl in Heq. destruct (def_closures B B0 rho1 H1 c l) as [H'' rho''] eqn:Hdef.
+    simpl in Heq. destruct (def_closures B B0 rho1 H1 l) as [H'' rho''] eqn:Hdef.
     destruct (alloc _ H'') as [l' H'''] eqn:Heq'.
     inv Heq. eapply well_formed_alloc; [| eassumption | ]; eauto.
-    simpl. rewrite Union_Empty_set_neut_r, Union_Empty_set_neut_l.
+    simpl. rewrite Union_Empty_set_neut_l.
     eapply Singleton_Included.
     eapply dom_subheap. eapply def_funs_subheap; eauto.
     eassumption.
@@ -1419,16 +1419,16 @@ Module HeapDefs (H : Heap).
       eexists; split; eauto. constructor.
   Qed.
 
-  Lemma well_formed_reach_def_closed_same (S : Ensemble loc) (H H' : heap block) B B0 rho rho' ct l :
+  Lemma well_formed_reach_def_closed_same (S : Ensemble loc) (H H' : heap block) B B0 rho rho' l :
     well_formed (reach' H S) H  ->
     In loc (dom H) l ->
     S \subset dom H ->
-    def_closures B B0 rho H ct l = (H', rho') ->
+    def_closures B B0 rho H l = (H', rho') ->
     reach' H S <--> reach' H' S.
   Proof.
     intros Hwf Hdom HS; revert H' rho'; induction B; intros H' rho' Hdef. 
     - simpl in Hdef.
-      destruct (def_closures B B0 rho H ct ) as [H'' rho''] eqn:Hdef'.
+      destruct (def_closures B B0 rho H l ) as [H'' rho''] eqn:Hdef'.
       destruct (alloc _ H'') as [l' H'''] eqn:Ha. inv Hdef.
       assert (Heq :reach' H'' S <--> reach' H' S).
       { eapply well_formed_reach_alloc_same; eauto.
@@ -1507,23 +1507,23 @@ Module HeapDefs (H : Heap).
         eapply env_locs_monotonic...
   Qed.
 
-  Lemma well_formed_reach_alloc_def_funs S H H' rho rho' B B0 l ct rho_clo :
+  Lemma well_formed_reach_alloc_def_funs S H H' rho rho' B B0 l rho_clo :
     well_formed (reach' H (env_locs rho S)) H ->
     env_locs rho S \subset dom H ->
     get l H = Some (Env rho_clo) ->
     env_locs rho_clo (Full_set _ ) \subset (reach' H (env_locs rho S)) ->
-    def_closures B B0 rho H ct l = (H', rho') ->
+    def_closures B B0 rho H l  = (H', rho') ->
     well_formed (reach' H' (env_locs rho' (Union _ S (name_in_fundefs B)))) H'.
   Proof with now eauto with Ensembles_DB.
     revert rho rho' H H'; induction B; intros rho rho' H H' Hwf Hsub Hget Hlocs Hdef; simpl.
     - simpl in Hdef.
-      destruct (def_closures B B0 rho H ct l) as [H'' rho''] eqn:Hdef'.
+      destruct (def_closures B B0 rho H l) as [H'' rho''] eqn:Hdef'.
       destruct (alloc _ H'') as [l' H'''] eqn:Hal. inv Hdef.
       rewrite (Union_commut [set v]), Union_assoc.
       eapply well_formed_reach_alloc_in_dom; [| | | eassumption |].
       + eapply IHB; eassumption.
       + eapply def_closures_env_locs_in_dom; eauto.
-      + simpl. rewrite Union_Empty_set_neut_l, Union_Empty_set_neut_r.
+      + simpl. rewrite Union_Empty_set_neut_l.
         rewrite post_Singleton with (b := Env rho_clo).
         * simpl. intros l1 Hin.
           eapply def_closures_post_reach. eassumption.
@@ -1533,7 +1533,7 @@ Module HeapDefs (H : Heap).
         * eapply def_funs_subheap; eauto.
       +  eapply Included_trans;
         [| now eapply dom_subheap; eapply def_funs_subheap; eauto ].
-         simpl. rewrite Union_Empty_set_neut_r, Union_Empty_set_neut_l.
+         simpl. rewrite Union_Empty_set_neut_l.
          eapply Singleton_Included. eexists; eauto.
     - inv Hdef. rewrite Union_Empty_set_neut_r. eassumption.
   Qed.
